Add preliminary contract transfer theorem depending on two unproven lemmas (#2)
* Add definition of multistep simulation (simulated_n_def) and refinement theorem (simulated_simulated_n)
* Change definition of contract simulation (simulated_contract_def)
* Add refinement theorem for contract simulation (simulated_simulated_contract) depending on two unproven lemmas about bir_exec_to_labels
* Add preliminary contract transfer theorem proved using theory above

examples/ijr/contractTransferScript.sml
@@ -1,53 +1,237 @@
 open HolKernel Parse boolLib bossLib;
 
-open bir_programTheory bir_htTheory;
+open listTheory;
+
+open bir_programTheory bir_htTheory bir_program_multistep_propsTheory;
 open HolBACoreSimps;
+
+open resolutionTheory simulationTheory;
 
 val _ = new_theory "contractTransfer";
 
 
-Definition contract_simulated_def:
-  contract_simulated p p' =
-  ∀s l ls s' o2 m2 n2.
-    s.bst_pc = bir_block_pc l ⇒
-    MEM l (bir_labels_of_program p) ⇒
-    (∀l'. l' IN ls ⇒ MEM l' (bir_labels_of_program p)) ⇒
-
-    bir_exec_to_labels ls p' s = BER_Ended o2 m2 n2 s' ⇒
-    ~(∃l'. s'.bst_status = BST_JumpOutside l') ⇒
-    (∃o1 m1 n1.
-      bir_exec_to_labels ls p s = BER_Ended o1 m1 n1 s')
+Definition exec_to_prog_n_def:
+  exec_to_prog_n p s pls n =
+  bir_exec_to_labels_n (set (bir_labels_of_program pls)) p s n
 End
 
+(*TODO: Strenthen simulation definitions wrt observations and steps?*)
+Definition simulated_n_def:
+  simulated_n p p' =
+  ∀n s l s' os2 m2 n2.
+    s.bst_pc = bir_block_pc l ⇒
+    MEM l (bir_labels_of_program p) ⇒
+
+    exec_to_prog_n p' s p n = BER_Ended os2 m2 n2 s' ⇒
+    ~(∃l'. s'.bst_status = BST_JumpOutside l') ⇒
+    (∃os1 m1 n1.
+      exec_to_prog_n p s p n = BER_Ended os1 m1 n1 s')
+End
+
+Theorem simulated_simulated_n:
+  ∀p p'. simulated p p' ⇒ simulated_n p p'
+Proof
+REPEAT STRIP_TAC >>
+SIMP_TAC std_ss [simulated_n_def, exec_to_prog_n_def] >>
+Q.ABBREV_TAC ‘ls = bir_labels_of_program p’ >>
+
+Induct_on ‘n’ >- (
+  SIMP_TAC (std_ss++holBACore_ss) [bir_exec_to_labels_n_REWR_0]
+) >>
+
+REPEAT GEN_TAC >> NTAC 2 STRIP_TAC >>
+SIMP_TAC (std_ss++holBACore_ss) [bir_exec_to_labels_n_REWR_SUC] >>
+
+(*Program p' takes a step*)
+Cases_on ‘bir_exec_to_labels (set ls) p' s’ >>
+SIMP_TAC (std_ss++holBACore_ss) [] >>
+rename1 ‘_ = BER_Ended os21 m21 n21 s2’ >>
+
+(*There is a contradiction or p takes the same step*)
+Cases_on ‘(∃l'. s2.bst_status = BST_JumpOutside l')’ >- (
+  FULL_SIMP_TAC (list_ss++holBACore_ss) [bir_state_is_terminated_def,
+                                         bir_exec_to_labels_n_REWR_TERMINATED] >>
+  STRIP_TAC >> FULL_SIMP_TAC (std_ss++holBACore_ss) []
+) >>
+subgoal ‘(∃os11 m11 n11.
+            bir_exec_to_labels (set ls) p s = BER_Ended os11 m11 n11 s2)’ >- (
+  FULL_SIMP_TAC (std_ss++holBACore_ss) [simulated_def, exec_to_prog_def]
+) >>
+ASM_SIMP_TAC (std_ss++holBACore_ss) [] >>
+
+(*If programs are terminated, rest of steps are same (needed to use induction hypothesis)*)
+Cases_on ‘(bir_state_is_terminated s2)’ >- (
+  FULL_SIMP_TAC (list_ss++holBACore_ss) [bir_state_is_terminated_def,
+                                         bir_exec_to_labels_n_REWR_TERMINATED]
+) >>
+
+(*Program p' takes the rest of the steps*)
+Cases_on ‘bir_exec_to_labels_n (set ls) p' s2 n’ >>
+SIMP_TAC (std_ss++holBACore_ss) [] >>
+rename1 ‘_ = BER_Ended os22 m22 n22 s2'’ >>
+NTAC 2 STRIP_TAC >>
+
+(*Program p takes the same rest of steps*)
+subgoal ‘∃os12 m12 n12.
+           bir_exec_to_labels_n (set ls) p s2 n = BER_Ended os12 m12 n12 s2'’ >- (
+  subgoal ‘∃l'. s2.bst_pc = bir_block_pc l' ∧ MEM l' ls’ >- (
+    MP_TAC (Q.SPECL [‘set ls’, ‘p'’, ‘s’, ‘os21’, ‘1’, ‘m21’, ‘n21’, ‘s2’]
+                    bir_exec_to_labels_n_ended_running) >>
+    FULL_SIMP_TAC (std_ss++holBACore_ss)
+                  [bir_block_pc_def, bir_exec_to_labels_def,
+                   bir_programcounter_t_component_equality]
+  ) >>
+  FULL_SIMP_TAC (std_ss++holBACore_ss) [exec_to_prog_n_def]
+) >>
+ASM_SIMP_TAC (std_ss++holBACore_ss) []
+QED
+
+Theorem bir_exec_to_labels_expand_labels:
+  ∀ls ls' p s s' os c1 c2.
+    ls SUBSET ls' ⇒
+    bir_exec_to_labels ls p s = BER_Ended os c1 c2 s' ⇒
+    (∃n c2'.
+       n > 0 ∧
+       bir_exec_to_labels_n ls' p s n = BER_Ended os c1 c2' s' ∧
+       (∀n'. 0 < n' ∧ n' < n ⇒
+             ∃s'' os' c1' c2''.
+               bir_exec_to_labels_n ls' p s n' = BER_Ended os' c1' c2'' s'' ∧
+               ~(s''.bst_pc.bpc_label IN ls)))
+Proof
+cheat
+QED
+
+Theorem bir_exec_to_labels_restrict_labels:
+  ∀ls ls' n p s s' os c1 c2.
+    ls SUBSET ls' ⇒
+    n > 0 ⇒
+    bir_exec_to_labels_n ls' p s n = BER_Ended os c1 c2 s' ⇒
+    s'.bst_pc.bpc_label IN ls ⇒
+    (∀n'. 0 < n' ∧ n' < n ⇒
+          ∃s'' os' c1' c2''.
+            bir_exec_to_labels_n ls' p s n' = BER_Ended os' c1' c2'' s'' ∧
+            ~(s''.bst_pc.bpc_label IN ls)) ⇒
+    (∃c2'. bir_exec_to_labels ls p s = BER_Ended os c1 c2' s')
+Proof
+cheat
+QED
+
+Definition simulated_contract_def:
+  simulated_contract p p' =
+  ∀s l ls s' os2 m2 n2.
+    s.bst_pc = bir_block_pc l ⇒
+    MEM l (bir_labels_of_program p) ⇒
+    ls SUBSET (set (bir_labels_of_program p)) ⇒
+
+    bir_exec_to_labels ls p' s = BER_Ended os2 m2 n2 s' ⇒
+    ~(bir_state_is_terminated s') ⇒
+    (∃os1 m1 n1.
+      bir_exec_to_labels ls p s = BER_Ended os1 m1 n1 s')
+End
+
+Theorem simulated_simulated_contract:
+  ∀p p'. simulated p p' ⇒ simulated_contract p p'
+Proof
+REPEAT STRIP_TAC >>
+SIMP_TAC std_ss [simulated_contract_def, exec_to_prog_n_def] >>
+Q.ABBREV_TAC ‘pls = bir_labels_of_program p’ >>
+
+(*Expand label set*)
+REPEAT STRIP_TAC >>
+MP_TAC (Q.SPECL [‘ls’, ‘set pls’, ‘p'’, ‘s’, ‘s'’, ‘os2’, ‘m2’, ‘n2’]
+                bir_exec_to_labels_expand_labels) >>
+ASM_SIMP_TAC std_ss [] >> STRIP_TAC >>
+rename1 ‘_ = BER_Ended _ _ n2' _’ >>
+
+(*Use simulation hypothesis*)
+subgoal ‘∃os1 m1 n1. bir_exec_to_labels_n (set pls) p s n =
+                     BER_Ended os1 m1 n1 s'’ >- (
+  subgoal ‘~(∃l'. s'.bst_status = BST_JumpOutside l')’ >- (
+    FULL_SIMP_TAC (std_ss++holBACore_ss) [bir_state_is_terminated_def]
+  ) >>
+  METIS_TAC [simulated_simulated_n, simulated_n_def, exec_to_prog_n_def]
+) >>
+
+(*Restrict label set*)
+subgoal ‘∃n1'.bir_exec_to_labels ls p s = BER_Ended os1 m1 n1' s'’ >- (
+  IRULE_TAC bir_exec_to_labels_restrict_labels >>
+  CONJ_TAC >- (
+    ‘(1:num) > 0’ by SIMP_TAC arith_ss [] >>
+    METIS_TAC [bir_exec_to_labels_def, bir_exec_to_labels_n_ended_running]
+  ) >>
+
+  Q.LIST_EXISTS_TAC [‘n1’, ‘set pls’, ‘n’] >> CONJ_TAC >- (
+    REPEAT STRIP_TAC >>
+    Q.PAT_X_ASSUM ‘∀n'. _’ (fn thm => ASSUME_TAC (Q.SPEC ‘n'’ thm)) >>
+    REV_FULL_SIMP_TAC std_ss [] >>
+
+    subgoal ‘~(∃l'. s''.bst_status = BST_JumpOutside l')’ >- (
+      FULL_SIMP_TAC std_ss [bir_exec_to_labels_n_def] >>
+      ‘~bir_state_is_terminated s''’ by
+        IMP_RES_TAC bir_exec_steps_GEN_decrease_max_steps_Ended_terminated >>
+      FULL_SIMP_TAC (std_ss++holBACore_ss) [bir_state_is_terminated_def]
+    ) >>
+    subgoal ‘∃os' c1' c2''. bir_exec_to_labels_n (set pls) p s n' =
+                            BER_Ended os' c1' c2'' s''’ >- (
+      METIS_TAC [simulated_simulated_n, simulated_n_def, exec_to_prog_n_def]
+    ) >>
+
+    PROVE_TAC []
+  ) >>
+
+  ASM_SIMP_TAC std_ss []
+) >>
+PROVE_TAC []
+QED
+
 Theorem contract_transfer:
-  ∀ (p' : 'a bir_program_t) l ls pre post  (p : 'a bir_program_t).
-    contract_simulated p p' ⇒
+  ∀ p p' l ls pre post.
+    simulated p p' ⇒
     bir_vars_of_program p' = bir_vars_of_program p ⇒
 
     MEM l (bir_labels_of_program p) ⇒
-    (∀l'. l' IN ls ⇒ MEM l' (bir_labels_of_program p)) ⇒
+    ls SUBSET (set (bir_labels_of_program p)) ⇒
 
     bir_exec_to_labels_triple p' l ls pre post ⇒
     bir_exec_to_labels_triple p l ls pre post
 Proof
 SIMP_TAC std_ss [bir_exec_to_labels_triple_def] >>
 REPEAT STRIP_TAC >>
+
+Q.PAT_X_ASSUM ‘simulated p p'’
+  (fn thm => ASSUME_TAC (MATCH_MP simulated_simulated_contract thm)) >>
+
 Q.PAT_X_ASSUM ‘∀s'. _’ (fn thm => ASSUME_TAC (Q.SPEC ‘s’ thm)) >>
 REV_FULL_SIMP_TAC std_ss [] >>
 rename1 ‘_ = BER_Ended o2 m2 n2 s'’ >>
 
-subgoal ‘∃s1 o1 m1 n1.
-           bir_exec_to_labels ls p s = BER_Ended o1 m1 n1 s'’ >- (
+subgoal ‘∃s1 o1 m1 n1. bir_exec_to_labels ls p s =
+                       BER_Ended o1 m1 n1 s'’ >- (
   ‘s.bst_pc = bir_block_pc l’ by (
     ASM_SIMP_TAC (std_ss++holBACore_ss)
-      [bir_block_pc_def, bir_programcounter_t_component_equality]
+                 [bir_block_pc_def,
+                  bir_programcounter_t_component_equality]
   ) >>
-  ‘~(∃l'. s'.bst_status = BST_JumpOutside l')’ by
-    ASM_SIMP_TAC (std_ss++holBACore_ss) [] >>
-  METIS_TAC [contract_simulated_def]
+  ‘~(bir_state_is_terminated s')’ by ASM_SIMP_TAC (std_ss++holBACore_ss) [] >>
+  METIS_TAC [simulated_contract_def]
 ) >>
 
 PROVE_TAC []
+QED
+
+(*Sanity check*)
+Theorem resolved_contract_transfer:
+  ∀l1 v sl p p' l ls pre post.
+    resolved l1 v sl p p' ⇒
+    bir_vars_of_program p' = bir_vars_of_program p ⇒
+
+    MEM l (bir_labels_of_program p) ⇒
+    ls SUBSET (set (bir_labels_of_program p)) ⇒
+
+    bir_exec_to_labels_triple p' l ls pre post ⇒
+    bir_exec_to_labels_triple p l ls pre post
+Proof
+PROVE_TAC [contract_transfer, resolved_simulated]
 QED
 
 
